%%%%%%%%%%%%%%%%%%%%%%%%%%%%%%%%%%%%%%%%%%%%%%%%%%%%%%%%%%%%%%%%%%%%%%%%%%%%%%%%
\section{Perturbation Theory}
\label{sec:bg:pert}
%%%%%%%%%%%%%%%%%%%%%%%%%%%%%%%%%%%%%%%%%%%%%%%%%%%%%%%%%%%%%%%%%%%%%%%%%%%%%%%%

Placeholder

%===============================================================================
\subsection{Greenspan}
\label{sec:bg:pert:greenspan}
%===============================================================================

Reference to Greenspan \cite{greenspan}.

% Equation 29
\begin{equation*}
  H\psi = q
\end{equation*}

% Equation 163
\begin{equation*}
  H^+\psi^+ = q^+
\end{equation*}

% Equation 44a
\begin{equation*}
  \bar{H}\delta\psi = \delta q - \delta H\psi
\end{equation*}

% Equation 44b
\begin{equation*}
  H\delta\psi = \delta q - \delta H\bar{\psi}
\end{equation*}

% Equation 164a
\begin{equation*}
  \bar{H}^+\delta\psi^+ = \bar{q}^+ - \bar{H}^+\psi^+ = \delta q^+ - \delta H^+\psi^+
\end{equation*}

% Equation 164b
\begin{equation*}
  H^+\delta\psi^+ = \delta q^+ - \delta H^+\bar{\psi}^+
\end{equation*}

% Equation 168
\begin{equation*}
  R = \left<\psi,q^+\right> = \left<\psi^+,q\right>
\end{equation*}

% Equation 169
\begin{equation*}
  R = \left<\psi,H^+\psi^+\right> = \left<\psi^+,H\psi\right>
\end{equation*}

% Equation 170a
\begin{equation*}\begin{split}
  \delta R = \bar{R} - R & = \left<\bar{\psi},\bar{q}^+\right> - \left<\psi,q^+\right> \\
                         & = \left<\psi,\delta q^+\right> + \left<\delta\psi,\bar{q}^+\right> \\
                         & = \left<\psi,\delta q^+\right> + \left<\bar{\psi}^+,\left(\delta q - \delta H\psi\right)\right>
\end{split}\end{equation*}

% Equation 170b
\begin{equation*}\begin{split}
  \delta R = \bar{R} - R & = \left<\bar{\psi}^+,\bar{q}\right> - \left<\psi^+,q\right> \\
                         & = \left<\psi^+,\delta q\right> + \left<\delta\psi^+,\bar{q}\right> \\
                         & = \left<\psi^+,\delta q\right> + \left<\bar{\psi},\left(\delta q^+ - \delta H^+\psi^+\right)\right>
\end{split}\end{equation*}

% Equation 171a, 171b
\begin{equation*}\begin{split}
  \delta R & = \delta R^{(1)} + \left<\delta\psi^+,\left(\delta q-\delta H\psi\right)\right> \\
           & = \delta R^{(1)} + \left<\delta\psi,\left(\delta q^+-\delta H^+\psi^+\right)\right>
\end{split}\end{equation*}

% Equation 172a, 172b
\begin{equation*}\begin{split}
  \delta R^{(1)} & = \left<\psi,\delta q^+\right> + \left<\psi^+,\left(\delta q - \delta H\psi\right)\right> \\
                 & = \left<\psi^+,\delta q\right> + \left<\psi,\left(\delta q^+ - \delta H^+\psi^+\right)\right>
\end{split}\end{equation*}

% Something about how this has been worked out for eigenvalue problems, but not for fixed source problems
